State pf to ir

src/pf2ir/PFtoIR.v
@@ -24,14 +24,112 @@ Require Import Global.
 Require Import Local.
 Require Import Thread.
 Require Import Configuration.
+Require Import PFConfiguration.
+Require Import Behavior.
 
 Require Import PFConsistent.
 Require Import FutureCertify.
 
 Set Implicit Arguments.
+Set Nested Proofs Allowed.
 
 
 Module PFtoIR.
+  Definition future_reserved (rsv: BoolMap.t) (reserved: TimeMap.t) (mem1 mem2: Memory.t): Prop :=
+    forall loc from to msg
+      (RESERVED: rsv loc = true)
+      (GET1: Memory.get loc to mem1 = None)
+      (GET2: Memory.get loc to mem2 = Some (from, msg)),
+      Time.lt (reserved loc) from.
+
+  Lemma future_reserved_trans
+        rsv reserved
+        mem1 mem2 mem3
+        (FUTURE12: Memory.future mem1 mem2)
+        (FUTURE23: Memory.future mem2 mem3)
+        (RESERVED12: future_reserved rsv reserved mem1 mem2)
+        (RESERVED23: future_reserved rsv reserved mem2 mem3):
+    future_reserved rsv reserved mem1 mem3.
+  Proof.
+    ii. destruct (Memory.get loc to mem2) as [[]|] eqn:GET; eauto.
+    exploit Memory.future_get1; try exact FUTURE23; try exact GET. i. des.
+    rewrite x0 in *. clarify. eauto.
+  Qed.
+
+  Lemma future_reserved_incr
+        rsv reserved1 reserved2 mem1 mem2
+        (INCR: TimeMap.le reserved2 reserved1)
+        (RESERVED: future_reserved rsv reserved1 mem1 mem2):
+    future_reserved rsv reserved2 mem1 mem2.
+  Proof.
+    ii. exploit RESERVED; eauto. i.
+    eapply TimeFacts.le_lt_lt; eauto.
+  Qed.
+
+  Lemma step_future_reserved
+        rsv
+        lang reserved pf e (th1 th2: Thread.t lang)
+        (RESERVED: BoolMap.le rsv (BoolMap.minus (Global.reserves (Thread.global th1))
+                                                 (Local.reserves (Thread.local th1))))
+        (STEP: Thread.step reserved pf e th1 th2):
+    future_reserved rsv reserved
+                    (Global.memory (Thread.global th1)) (Global.memory (Thread.global th2)).
+  Proof.
+    ii. inv STEP; inv STEP0; ss; try congr; try by (inv LOCAL; ss; congr).
+    - inv LOCAL. ss.
+      revert GET2. erewrite Memory.add_o; eauto. condtac; ss; try congr.
+      i. des. inv GET2.
+      exploit RESERVED; eauto.
+      unfold BoolMap.minus.
+      destruct (Global.reserves gl1 loc0), (Local.reserves lc1 loc0); ss. i. eauto.
+    - inv LOCAL1. inv LOCAL2. ss.
+      revert GET2. erewrite Memory.add_o; eauto. condtac; ss; try congr.
+      i. des. inv GET2.
+      exploit RESERVED; eauto.
+      unfold BoolMap.minus.
+      destruct (Global.reserves gl1 loc0), (Local.reserves lc1 loc0); ss. i. eauto.
+  Qed.
+
+  Lemma rtc_all_step_future_reserved
+        rsv
+        lang reserved (th1 th2: Thread.t lang)
+        (LC_WF: Local.wf (Thread.local th1) (Thread.global th1))
+        (GL_WF: Global.wf (Thread.global th1))
+        (RESERVED: BoolMap.le rsv (BoolMap.minus (Global.reserves (Thread.global th1))
+                                                 (Local.reserves (Thread.local th1))))
+        (STEPS: rtc (@Thread.all_step lang reserved) th1 th2):
+    future_reserved rsv reserved
+                    (Global.memory (Thread.global th1)) (Global.memory (Thread.global th2)).
+  Proof.
+    revert RESERVED. induction STEPS; i.
+    { ii. congr. }
+    inv H. inv USTEP.
+    hexploit step_future_reserved; try exact STEP; eauto. i.
+    exploit Thread.step_future; try exact STEP0; eauto. i. des.
+    exploit Thread.rtc_all_step_future; try exact STEPS; eauto. i. des.
+    exploit Thread.step_reserves_minus; eauto. i.
+    rewrite x1 in *.
+    hexploit IHSTEPS; eauto. i.
+    eapply future_reserved_trans; try exact H; ss;
+      try apply GL_FUTURE; try apply GL_FUTURE0.
+  Qed.
+
+  Lemma rtc_tau_step_future_reserved
+        rsv
+        lang reserved (th1 th2: Thread.t lang)
+        (LC_WF: Local.wf (Thread.local th1) (Thread.global th1))
+        (GL_WF: Global.wf (Thread.global th1))
+        (RESERVED: BoolMap.le rsv (BoolMap.minus (Global.reserves (Thread.global th1))
+                                                 (Local.reserves (Thread.local th1))))
+        (STEPS: rtc (@Thread.tau_step lang reserved) th1 th2):
+    future_reserved rsv reserved
+                    (Global.memory (Thread.global th1)) (Global.memory (Thread.global th2)).
+  Proof.
+    eapply rtc_all_step_future_reserved; eauto.
+    eapply rtc_implies; try exact STEPS.
+    i. inv H. inv TSTEP. econs; eauto.
+  Qed.
+
   Variant sim_thread_sl (gl_pf gl_ir: Global.t):
     forall (sl_pf sl_ir: {lang: language & Language.state lang} * Local.t), Prop :=
     | sim_thread_sl_intro
@@ -46,7 +144,16 @@ Module PFtoIR.
         (GPROMISES: Global.promises gl_pf = BoolMap.bot)
         (GRESERVES: Global.reserves gl_pf = BoolMap.bot)
         (MEMORY: Global.memory gl_pf = Global.memory gl_ir)
-      : sim_thread_sl gl_pf gl_ir (existT _ lang st_pf, lc_pf) (existT _ lang st_ir, lc_ir)
+        (CONS: exists gl_past,
+            (<<FUTURE: Global.future gl_past gl_ir>>) /\
+            (<<RESERVED: future_reserved
+                           (Local.reserves lc_ir) (Memory.max_timemap (Global.memory gl_past))
+                           (Global.memory gl_past) (Global.memory gl_ir)>>) /\
+            (<<LC_WF: Local.wf lc_ir gl_past>>) /\
+            (<<GL_WF: Global.wf gl_past>>) /\
+            (<<CONS: PFConsistent.spf_consistent (Thread.mk _ st_ir lc_ir gl_past)>>))
+      :
+      sim_thread_sl gl_pf gl_ir (existT _ lang st_pf, lc_pf) (existT _ lang st_ir, lc_ir)
   .
 
   Variant sim_conf: forall (c_pf c_ir: Configuration.t), Prop :=
@@ -60,4 +167,59 @@ Module PFtoIR.
               (IdentMap.find tid ths_ir)):
       sim_conf (Configuration.mk ths_pf gl_pf) (Configuration.mk ths_ir gl_ir)
   .
+
+  Lemma init_sim_conf prog: sim_conf (Configuration.init prog) (Configuration.init prog).
+  Proof.
+    econs. i.
+    unfold Threads.init. rewrite IdentMap.Facts.map_o.
+    destruct (@UsualFMapPositive.UsualPositiveMap'.find
+                (@sigT _ (@Language.syntax ProgramEvent.t)) tid prog); ss.
+    econs; ss.
+    exists Global.init. splits.
+    - refl.
+    - ii. ss.
+    - apply Local.init_wf.
+    - apply Global.init_wf.
+    - econs 2; s; try refl.
+  Qed.
+
+  Lemma sim_conf_terminal
+        c1_pf c1_ir
+        (SIM: sim_conf c1_pf c1_ir)
+        (TERMINAL: Configuration.is_terminal c1_ir):
+    Configuration.is_terminal c1_pf.
+  Proof.
+    inv SIM. ii. ss.
+    specialize (THS tid). rewrite FIND in THS.
+    destruct (IdentMap.find tid ths_ir) as [[[lang_ir st_ir] lc_ir]|] eqn:FIND_IR; ss.
+    inv THS. Configuration.simplify. splits; ss.
+    exploit TERMINAL; eauto. i. des. ss.
+  Qed.
+
+  Lemma sim_conf_step
+        c1_pf c1_ir
+        e tid c2_ir
+        (SIM: sim_conf c1_pf c1_ir)
+        (WF1_PF: Configuration.wf c1_pf)
+        (WF1_IR: Configuration.wf c1_ir)
+        (STEP: Configuration.step e tid c1_ir c2_ir):
+    (exists c_pf c2_pf,
+        (<<STEPS_PF: rtc (PFConfiguration.tau_step ThreadEvent.get_machine_event_pf)
+                         c1_pf c_pf>>) /\
+        (<<STEP_PF: PFConfiguration.step ThreadEvent.get_machine_event_pf
+                                         MachineEvent.failure tid c_pf c2_pf>>)) \/
+    (exists c_pf c2_pf,
+        (<<STEPS_PF: rtc (PFConfiguration.tau_step ThreadEvent.get_machine_event_pf)
+                         c1_pf c_pf>>) /\
+        (<<STEP_PF: PFConfiguration.opt_step ThreadEvent.get_machine_event_pf
+                                             e tid c_pf c2_pf>>) /\
+        (<<SIM2: sim_conf c2_pf c2_ir>>)).
+  Proof.
+  Admitted.
+
+  Theorem pf_to_ir prog:
+    behaviors Configuration.step (Configuration.init prog) <2=
+    behaviors (PFConfiguration.step ThreadEvent.get_machine_event_pf) (Configuration.init prog).
+  Proof.
+  Admitted.
 End PFtoIR.
